---
date: 2010-05-15T16:29:01+00:00
layout: page
---
The sum \\\(S\\) of the geometric progression with \\(n\\) terms, ratio \\(r\\) and first term \\(a\\)

$$ S = a + a r + a r^2 + a r^3 + \ldots + a r^{n-2} + a r^{n-1} $$

is calculated buy multiplying the equation above by \\(r\\) to obtain

$$ r S = a r + a r^2 + a r^3 + \ldots + a r^{n-1} + a r^n $$

And then subtracting the top equation from the bottom one to obtain

$$

\begin{eqnarray*}

r S - S & = \;\;\;\; & & a r & + a r^2 \;+ a r^3 \;+ \ldots \;+ a r^{n-1} \;+ a r^n \\
        &   - a & & - a r & - a r^2 - a r^3 - \ldots - a r^{n-1}

\end{eqnarray*}

$$

On the right, all but two terms cancel out and we get

$$

\begin{eqnarray*}

r S - S & = & a r^n - a \\

S ( r - 1 ) & = & a ( r^n - 1 ) \\

& & \\

S & = & a \frac{r^n - 1}{r-1}

\end{eqnarray*}

$$
